Move results on partial memories to Memory
Complete the library of existing results on partial memories in the
Memory module by relocating there the additions found elsewhere, mostly
in the intermediate PS.

Given their location there, it is natural to include the definitions for
partialization and combination of memories instead of employing
explicit and more cumbersom filterm operations.

At the moment, some derived results and notions of memory merging proper
to Recombination remain there.

Common/Memory.v
@@ -271,6 +271,12 @@ Unset Printing Implicit Defensive.
 
 (* TODO: Clean these lemmas and their weak variants *)
 
+Definition to_partial_memory (mem : Memory.t) (ctx : {fset Component.id}) :=
+  filterm (fun k _ => negb (k \in ctx)) mem.
+
+Definition merge_memories (mem1 mem2: Memory.t): Memory.t :=
+  unionm mem1 mem2.
+
 Lemma program_allocation_in_partialized_memory_strong :
   forall (ctx: {fset Component.id}) mem1 mem2,
     filterm (fun k _ => k \notin ctx) mem1 =
@@ -291,7 +297,6 @@ eexists; eauto; apply/eq_fmap=> C'; rewrite !filtermE !setmE.
 case: eqP=> [-> {C'}|_] //=.
 by move/(_ C'): Hfilter; rewrite !filtermE.
 Qed.
-
 
 Lemma program_allocation_in_partialized_memory:
   forall (ctx: {fset Component.id}) mem1 mem2,
@@ -416,4 +421,112 @@ Proof.
   rewrite filtermE filtermE setmE.
   case: (@eqP _ C' C) => [-> | _] //.
   by rewrite C_in_ctx mem_C /=.
+Qed.
+
+(* RB: TODO: More properly, this seems to belong in Machine.Memory. However, it
+   is natural to resort to a notion of partial memory that seems logically
+   related to the supporting components of PS. Again, note, however, that this
+   notion of partial memory is already used in the Memory module, and it may be
+   a good idea to relocate our compact definitions there.
+
+   Otherwise, this is a more convenient wrapper for
+   context_store_in_partialized_memory which does not require the destruction of
+   pointers, and could conceivably replace the wrappee throughout the
+   development. *)
+Lemma program_store_to_partialized_memory
+      ptr (iface : Program.interface) mem mem' v :
+  Pointer.component ptr \in domm iface ->
+  Memory.store mem ptr v = Some mem' ->
+  to_partial_memory mem (domm iface) = to_partial_memory mem' (domm iface).
+Proof.
+  destruct ptr as [[C b] o]. simpl.
+  intros Hdome Hsome.
+  unfold to_partial_memory. symmetry.
+  eapply context_store_in_partialized_memory; eassumption.
+Qed.
+
+(* RB: TODO: Same notes as above.
+   Cf.  program_allocation_in_partialized_memory_strong. *)
+Lemma program_allocation_to_partialized_memory
+      C (iface : Program.interface) size mem mem' ptr :
+  C \in domm iface ->
+  Memory.alloc mem C size = Some (mem', ptr) ->
+  to_partial_memory mem (domm iface) = to_partial_memory mem' (domm iface).
+Proof.
+  destruct ptr as [[C' b] o]. simpl.
+  intros Hdome Hsome.
+  unfold to_partial_memory. symmetry.
+  eapply context_allocation_in_partialized_memory; eassumption.
+Qed.
+
+(* The following two lemmas manipulate memory stores and partialized memories
+   more conveniently than the full-fledged "partialized" results. Note naming
+   conventions for some of those are currently somewhat confusing.  *)
+Lemma partialize_program_store :
+  forall mem mem' (ctx : Program.interface) ptr v,
+    Pointer.component ptr \notin domm ctx ->
+    Memory.store mem ptr v = Some mem' ->
+    Memory.store (to_partial_memory mem (domm ctx)) ptr v =
+    Some (to_partial_memory mem' (domm ctx)).
+Proof.
+  unfold Memory.store, to_partial_memory.
+  intros mem mem' ctx ptr v Hnotin Hstore.
+  destruct (mem (Pointer.component ptr)) as [memC |] eqn:HmemC;
+    last discriminate.
+  destruct (ComponentMemory.store memC (Pointer.block ptr) (Pointer.offset ptr) v)
+    as [memC' |] eqn:HmemC';
+    last discriminate.
+  inversion Hstore as [[Hstore']].
+  now rewrite (getm_filterm_notin_domm _ Hnotin) HmemC HmemC'
+      (setm_filterm_notin_domm _ _ Hnotin).
+Qed.
+
+Lemma unpartialize_program_store :
+  forall mem1 mem1' mem2 ptr v,
+    Memory.store mem1 ptr v = Some mem1' ->
+    Memory.store (merge_memories mem1 mem2) ptr v =
+    Some (merge_memories mem1' mem2).
+Proof.
+  unfold Memory.store.
+  intros mem1 mem1' mem2 ptr v Hstore.
+  unfold merge_memories. rewrite unionmE.
+  destruct (mem1 (Pointer.component ptr)) eqn:Hcase1; rewrite Hcase1;
+    last discriminate.
+  simpl.
+  destruct (ComponentMemory.store t (Pointer.block ptr) (Pointer.offset ptr) v) eqn:Hcase2;
+    last discriminate.
+  rewrite setm_union. now inversion Hstore.
+Qed.
+
+Lemma partialize_program_alloc :
+  forall mem mem' (ctx : Program.interface) C ptr size,
+    C \notin domm ctx ->
+    Memory.alloc mem C size = Some (mem', ptr) ->
+    Memory.alloc (to_partial_memory mem (domm ctx)) C size =
+    Some (to_partial_memory mem' (domm ctx), ptr).
+Proof.
+  unfold Memory.alloc, to_partial_memory.
+  intros mem mem' ctx C ptr size Hnotin Halloc.
+  destruct (mem C) as [memC |] eqn:HmemC;
+    last discriminate.
+  destruct (ComponentMemory.alloc memC size) as [memC' b] eqn:HmemC'.
+  inversion Halloc; subst.
+  now rewrite (getm_filterm_notin_domm _ Hnotin) HmemC HmemC'
+      (setm_filterm_notin_domm _ _ Hnotin).
+Qed.
+
+Lemma unpartialize_program_alloc :
+  forall mem1 mem1' mem2 C ptr size,
+    Memory.alloc mem1 C size = Some (mem1', ptr) ->
+    Memory.alloc (merge_memories mem1 mem2) C size =
+    Some (merge_memories mem1' mem2, ptr).
+Proof.
+  unfold Memory.alloc.
+  intros mem1 mem1' mem2 C ptr size Halloc.
+  unfold merge_memories. rewrite unionmE.
+  destruct (mem1 C) as [memC |] eqn:Hcase1; rewrite Hcase1;
+    last discriminate.
+  simpl.
+  destruct (ComponentMemory.alloc memC size) as [memC' b].
+  rewrite setm_union. now inversion Halloc.
 Qed.
